# Infix to Postfix Conversion

This repository provides a Java implementation to convert a given infix expression to a postfix expression. The algorithm ensures operator precedence and correct handling of parentheses for accurate conversion.

## Table of Contents

- [Introduction](#introduction)
- [Algorithm](#algorithm)
- [Operator Precedence](#operator-precedence)
- [Usage](#usage)
- [Example Input/Output](#example-inputoutput)
- [Code](#code)

## Introduction

Infix expressions are standard algebraic notations (e.g., `a+b`). To evaluate such expressions using stacks, we convert them into postfix expressions (e.g., `ab+`). This project provides a step-by-step implementation of this conversion in Java.

## Algorithm

1. **Initialize**:
   - Use a stack to hold operators and parentheses.

2. **Iterate through the infix expression**:
   - Append operands directly to the output.
   - Push '(' onto the stack.
   - Pop operators to the output until '(' is found for ')'.
   - Handle operators based on precedence based on:
     - The stack is not empty.
     - The top of the stack has higher or equal precedence than the current operator. Push the current operator onto the stack.

3. **After traversal**:
   - Append all remaining operators in the stack to the output.

## Operator Precedence

| Operator | Precedence |
|----------|------------|
| `^`      | Highest    |
| `*`, `/` | Medium     |
| `+`, `-` | Lowest     |

## Usage

1. Clone the repository.
2. Compile and run the Java code using:
   ```bash
   javac InfixToPostfix.java
   java InfixToPostfix
   ```
3. Modify the `main` method for custom input expressions.

## Example Input/Output

### Example 1
**Input:** `a+b*(c^d-e)^(f+g*h)-i`  
**Output:** `abcd^e-fgh*+^*+i-`

### Example 2
**Input:** `(p+q)*(m-n)`  
**Output:** `pq+mn-*`

## Code

```java
import java.util.Stack;

public class InfixToPostfix {

    // Method to return precedence of operators
    private static int precedence(char operator) {
        switch (operator) {
            case '^':
                return 3;
            case '*':
            case '/':
                return 2;
            case '+':
            case '-':
                return 1;
            default:
                return -1;
        }
    }

    // Method to convert infix to postfix
    public static String infixToPostfix(String expression) {
        StringBuilder postfix = new StringBuilder();
        Stack<Character> stack = new Stack<>();

        for (int i = 0; i < expression.length(); i++) {
            char ch = expression.charAt(i);

            if (Character.isLetterOrDigit(ch)) {
                postfix.append(ch);
            }
            // If the character is '(', push it to the stack
            else if (ch == '(') {
                stack.push(ch);
            }
            // If the character is ')', pop until '(' is found
            else if (ch == ')') {
                while (!stack.isEmpty() && stack.peek() != '(') {
                    postfix.append(stack.pop());
                }
                stack.pop(); // Remove '(' from stack
            }
            // If the character is an operator
            else {
                while (!stack.isEmpty() && precedence(stack.peek()) >= precedence(ch)) {
                    postfix.append(stack.pop());
                }
                stack.push(ch);
            }
        }

        // Pop all the operators left in the stack
        while (!stack.isEmpty()) {
            postfix.append(stack.pop());
        }

        return postfix.toString();
    }

    public static void main(String[] args) {
        String infix1 = "a+b*(c^d-e)^(f+g*h)-i";
        String infix2 = "(p+q)*(m-n)";
        System.out.println("Postfix of '" + infix1 + "' : " + infixToPostfix(infix1));
        System.out.println("Postfix of '" + infix2 + "' : " + infixToPostfix(infix2));
    }
}
```

------

### Example 1: `a+b*(c^d-e)^(f+g*h)-i`
| Step | Symbol | Action | Stack | Postfix Expression |
|------|--------|--------|--------|---------------------|
| 1 | a | Operand → Add to postfix | [] | "a" |
| 2 | + | Operator → Push to stack | [+] | "a" |
| 3 | b | Operand → Add to postfix | [+] | "ab" |
| 4 | * | Operator → Push to stack | [+, *] | "ab" |
| 5 | ( | Left parenthesis → Push | [+, *, (] | "ab" |
| 6 | c | Operand → Add to postfix | [+, *, (] | "abc" |
| 7 | ^ | Operator → Push | [+, *, (, ^] | "abc" |
| 8 | d | Operand → Add to postfix | [+, *, (, ^] | "abcd" |
| 9 | - | Operator → Pop ^, push - | [+, *, (, -] | "abcd^" |
| 10 | e | Operand → Add to postfix | [+, *, (, -] | "abcd^e" |
| 11 | ) | Right parenthesis → Pop - | [+, *] | "abcd^e-" |
| 12 | ^ | Operator → Push | [+, *, ^] | "abcd^e-" |
| 13 | ( | Left parenthesis → Push | [+, *, ^, (] | "abcd^e-" |
| 14 | f | Operand → Add to postfix | [+, *, ^, (] | "abcd^e-f" |
| 15 | + | Operator → Push | [+, *, ^, (, +] | "abcd^e-f" |
| 16 | g | Operand → Add to postfix | [+, *, ^, (, +] | "abcd^e-fg" |
| 17 | * | Operator → Push | [+, *, ^, (, +, *] | "abcd^e-fg" |
| 18 | h | Operand → Add to postfix | [+, *, ^, (, +, *] | "abcd^e-fgh" |
| 19 | ) | Right parenthesis → Pop *, + | [+, *, ^] | "abcd^e-fgh*+" |
| 20 | ) | Right parenthesis → Pop ^ | [+, *] | "abcd^e-fgh*+^" |
| 21 | - | Operator → Pop *, + then push - | [-] | "abcd^e-fgh*+^*+" |
| 22 | i | Operand → Add to postfix | [-] | "abcd^e-fgh*+^*+i" |
| 23 | End | Pop remaining - from stack | [] | "abcd^e-fgh*+^*+i-" |

**Final Postfix Expression:** `abcd^e-fgh*+^*+i-`

### Example 2: `(p+q)*(m-n)`
| Step | Symbol | Action | Stack | Postfix Expression |
|------|--------|--------|--------|---------------------|
| 1 | ( | Left parenthesis → Push | [(] | "" |
| 2 | p | Operand → Add to postfix | [(] | "p" |
| 3 | + | Operator → Push | [(, +] | "p" |
| 4 | q | Operand → Add to postfix | [(, +] | "pq" |
| 5 | ) | Right parenthesis → Pop + | [] | "pq+" |
| 6 | * | Operator → Push | [*] | "pq+" |
| 7 | ( | Left parenthesis → Push | [*, (] | "pq+" |
| 8 | m | Operand → Add to postfix | [*, (] | "pq+m" |
| 9 | - | Operator → Push | [*, (, -] | "pq+m" |
| 10 | n | Operand → Add to postfix | [*, (, -] | "pq+mn" |
| 11 | ) | Right parenthesis → Pop - | [*] | "pq+mn-" |
| 12 | End | Pop remaining * from stack | [] | "pq+mn-*" |
